src/PFuncAbstractDomain.v
@@ -1,75 +1,132 @@
 From Coq Require Import ssreflect ssrfun ssrbool.
 From Coq Require Import ssrbool Ensembles.
 From PolyAI Require Export PFunc LSSA AbstractDomain.
+Local Set Warnings "-notation-overridden".
+From mathcomp Require Import ssrnat eqtype.
 
 Local Open Scope string_scope.
 
-Section PFuncAbstractDomain.
-
-  Context {PMap PSet PwAff: eqType}
-          {PI: PresburgerImpl PMap PSet PwAff}.
+Module PFuncMap (FPI: FPresburgerImpl).
+  Import FPI.
+  Module PFI := PFuncImpl FPI.
+  Import PFI.
 
   Definition concrete_state := prod_eqType RegisterMap RegisterMap.
 
-  Definition PFuncMap := @total_map_eqType string_eqType (@PFunc_eqType PSet PwAff).
+  Definition to_var_values_seq (p: Program) (R: RegisterMap) :=
+    List.map (fun v => R v) (vars_in_program p).
 
-  Definition bot_PFuncMap : PFuncMap :=
-    (_ !-> constant_pfunc VBot).
+  Definition PFuncMap (p: Program) :=
+    let n := size (vars_in_program p) in
+    { x: seq (PFunc_eqType n) | size x == n}.
 
-  Definition top_PFuncMap : PFuncMap :=
-    (_ !-> constant_pfunc VTop).
+  Program Definition bot_PFuncMap (p: Program) : PFuncMap p :=
+    let n := size (vars_in_program p) in
+    (nseq n (constant_pfunc n VBot)).
+  Next Obligation.
+      by rewrite size_nseq.
+  Qed.
 
-  Definition join_PFuncMap (p1 p2: PFuncMap) :=
-    t_pointwise_bin_op p1 p2 (fun x1 x2 => join_pfunc x1 x2).
+  Program Definition top_PFuncMap (p: Program) : PFuncMap p :=
+    let n := size (vars_in_program p) in
+    nseq n (constant_pfunc n VTop).
+  Next Obligation.
+      by rewrite size_nseq.
+  Qed.
 
-  Definition gamma_PFuncMap (p: PFuncMap) :=
-    fun (x: concrete_state) => forall i, in_V (x.2 i) (eval_pfunc (p i) x.1).
+  Program Definition join_PFuncMap {p: Program} (p1 p2: PFuncMap p) : PFuncMap p :=
+    [ seq join_pfunc x.1 x.2 | x <- zip p1 p2].
+  Next Obligation.
+    rewrite size_map size_zip.
+    case: p1. case: p2.
+    move => x /eqP -> x0 /eqP ->.
+      by rewrite ssrnat.minnn.
+  Qed.
+
+  Definition gamma_PFuncMap {p: Program} (pf: PFuncMap p) (x: concrete_state) :=
+    let inputs := to_var_values_seq p x.1 in
+    forall i, (x.2 (nth "" (vars_in_program p) i)) \inV (eval_pfunc (nth (constant_pfunc _ VTop) (sval pf) i) inputs).
 
   Theorem gamma_top_PFuncMap :
-    forall x, Ensembles.In _ (gamma_PFuncMap top_PFuncMap) x.
+    forall p x, Ensembles.In _ (gamma_PFuncMap (top_PFuncMap p)) x.
   Proof.
-    move => x. rewrite /In /gamma_PFuncMap /top_PFuncMap.
-    by auto_pfunc.
+    move => p x var_values i. rewrite /In /gamma_PFuncMap /top_PFuncMap nth_nseq.
+    case_if; auto_pfunc.
   Qed.
 
   Theorem gamma_bot_PFuncMap :
-    forall x, ~ Ensembles.In _ (gamma_PFuncMap bot_PFuncMap) x.
+    forall p x, ~ Ensembles.In _ (gamma_PFuncMap (bot_PFuncMap p)) x.
   Proof.
-    rewrite /In /gamma_PFuncMap /bot_PFuncMap => x /(_ "").
-    by simpl_pfunc.
+    rewrite /In /gamma_PFuncMap /bot_PFuncMap => p x /(_ 0). rewrite nth_nseq.
+    case_if. by simpl_pfunc.
+      by rewrite size_vars_in_program in H.
   Qed.
 
-  Theorem join_sound_l_PFuncMap :
-    forall a1 a2, Included _ (gamma_PFuncMap a1) (gamma_PFuncMap (join_PFuncMap a1 a2)).
-  Proof.
-    rewrite /Included /In /gamma_PFuncMap /join_PFuncMap => a1 a2 x Hle s.
-    move => /(_ s) in Hle. move: Hle. simpl_pfunc.
-    apply le_V_spec.
-      by auto_pfunc.
-  Qed.
+    Theorem join_sound_l_PFuncMap :
+      forall p a1 a2, Included _ (@gamma_PFuncMap p a1) (gamma_PFuncMap (join_PFuncMap a1 a2)).
+    Proof.
+      rewrite /Included /In /gamma_PFuncMap /join_PFuncMap => p [a1 size_a1] [a2 size_a2].
+      move: (size_a1) (size_a2).
+      move => /eqP in size_a1. move => /eqP in size_a2.
+      move => size_a1' size_a2' x Hle i.
+      move => /(_ i) in Hle. move: Hle. simpl_pfunc.
+      apply le_V_spec.
+      case Hs : (i < size a1).
+      - erewrite nth_map; last first. by rewrite size_zip size_a1 size_a2 minnn -size_a1.
+        erewrite nth_zip; last first. by rewrite size_a1 size_a2.
+        rewrite /= join_pfuncP.
+          by apply join_V_leftP.
+      - rewrite !nth_default.
+        + by apply le_V_refl.
+        + rewrite size_map size_zip size_a1 size_a2 minnn -size_a1.
+            by rewrite leqNgt Hs.
+        + by rewrite leqNgt Hs.
+    Unshelve.
+      eapply constant_pfunc.
+      by apply VTop.
+    Qed.
 
-  Theorem join_sound_r_PFuncMap :
-    forall a1 a2, Included _ (gamma_PFuncMap a2) (gamma_PFuncMap (join_PFuncMap a1 a2)).
-  Proof.
-    rewrite /Included /In /gamma_PFuncMap /join_PFuncMap => a1 a2 x Hle s.
-    move => /(_ s) in Hle. move: Hle. simpl_pfunc.
-    apply le_V_spec.
-    by auto_pfunc.
-  Qed.
+    Theorem join_sound_r_PFuncMap :
+      forall p a1 a2, Included _ (@gamma_PFuncMap p a2) (gamma_PFuncMap (join_PFuncMap a1 a2)).
+    Proof.
+      rewrite /Included /In /gamma_PFuncMap /join_PFuncMap => p [a1 size_a1] [a2 size_a2].
+      move: (size_a1) (size_a2).
+      move => /eqP in size_a1. move => /eqP in size_a2.
+      move => size_a1' size_a2' x Hle i.
+      move => /(_ i) in Hle. move: Hle. simpl_pfunc.
+      apply le_V_spec.
+      case Hs : (i < size a2).
+      - erewrite nth_map; last first. by rewrite size_zip size_a1 size_a2 minnn -size_a2.
+        erewrite nth_zip; last first. by rewrite size_a1 size_a2.
+        rewrite /= join_pfuncP.
+          by apply join_V_rightP.
+      - rewrite !nth_default.
+        + by apply le_V_refl.
+        + rewrite size_map size_zip size_a1 size_a2 minnn -size_a2.
+            by rewrite leqNgt Hs.
+        + by rewrite leqNgt Hs.
+          Unshelve.
+          eapply constant_pfunc.
+            by apply VTop.
+    Qed.
 
-  Instance adom_pmap : adom concrete_state PFuncMap :=
+    Definition PFuncMap_eqMixin (p: Program) :=
+      let n := size (vars_in_program p) in
+      @sig_eqMixin (seq_eqType (PFunc_eqType n)) (fun x => size x == n).
+    Canonical PFuncMap_eqType (p: Program) := Eval hnf in EqType (PFuncMap p) (PFuncMap_eqMixin p).
+
+  Instance adom_pmap (p: Program) : adom concrete_state (PFuncMap_eqType p) p :=
     {
-      bot := bot_PFuncMap;
-      top := top_PFuncMap;
+      bot := bot_PFuncMap p;
+      top := top_PFuncMap p;
       join := join_PFuncMap;
 
       gamma := gamma_PFuncMap;
 
-      gamma_top := gamma_top_PFuncMap;
-      gamma_bot := gamma_bot_PFuncMap;
-      join_sound_l := join_sound_l_PFuncMap;
-      join_sound_r := join_sound_r_PFuncMap;
+      gamma_top := gamma_top_PFuncMap p;
+      gamma_bot := gamma_bot_PFuncMap p;
+      join_sound_l := join_sound_l_PFuncMap p;
+      join_sound_r := join_sound_r_PFuncMap p;
     }.
 
-
-End PFuncAbstractDomain.
+End PFuncMap.
