src/FinitePresburger.v
@@ -44,17 +44,17 @@ Module Type FPresburgerImpl.
   Parameter f_union_set: forall n, PSet n -> PSet n -> PSet n.
   Arguments f_union_set {n}.
   Axiom f_union_setP: forall n (p1 p2: PSet n) x,
-      x \ins (f_union_set p1 p2) -> (x \ins p1) || (x \ins p2).
+      x \ins (f_union_set p1 p2) = (x \ins p1) || (x \ins p2).
 
   Parameter f_intersect_set: forall n, PSet n -> PSet n -> PSet n.
   Arguments f_intersect_set {n}.
   Axiom f_intersect_setP: forall n (p1 p2: PSet n) x,
-      x \ins (f_intersect_set p1 p2) -> (x \ins p1) && (x \ins p2).
+      x \ins (f_intersect_set p1 p2) = (x \ins p1) && (x \ins p2).
 
   Parameter f_subtract_set: forall n, PSet n -> PSet n -> PSet n.
   Arguments f_subtract_set {n}.
   Axiom f_subtract_setP: forall n (p1 p2: PSet n) x,
-      x \ins (f_subtract_set p1 p2) -> (x \ins p1) && ~~ (x \ins p2).
+      x \ins (f_subtract_set p1 p2) = (x \ins p1) && ~~ (x \ins p2).
 
   Parameter f_is_subset_set: forall n, PSet n -> PSet n -> bool.
   Arguments f_is_subset_set {n}.
@@ -217,7 +217,14 @@ Module Type FPresburgerImpl.
   Axiom f_get_involved_dimP :
     forall n (p: PwAff n) d, d \in (f_get_involved_dim p) = f_involves_dim_pw_aff p d.
 
-  Hint Rewrite @f_universe_setP @f_union_setP @f_intersect_setP
+  Theorem f_empty_set_rw :
+    forall n x, x \ins (f_empty_set n) = false.
+  Proof.
+    move => n x.
+      by rewrite (negbTE (f_empty_setP _ _)).
+  Qed.
+
+  Hint Rewrite @f_empty_set_rw @f_universe_setP @f_union_setP @f_intersect_setP
        @f_subtract_setP @f_apply_range_mapP
        @f_universe_mapP @f_id_mapP @f_union_mapP @f_intersect_mapP
        @f_pw_aff_from_affP @f_intersect_domainP @f_union_pw_affP @f_eq_setP @f_ne_setP @f_le_setP @f_indicator_functionP
